new/golang/defn/predeclared.v
@@ -560,6 +560,9 @@ Class PredeclaredSemantics `{!GoSemanticsFunctions} :=
   make2_underlying t : functions make2 [t] = functions make2 [underlying t];
   make1_underlying t : functions make1 [t] = functions make1 [underlying t];
 
+  (* TODO: these should be FuncUnfold instances.
+     Write and prove specs that cover the cases for max() of two uint64s in theory/predeclared.v.
+   *)
   min_ordered n t : #(functions min (replicate n t)) = minⁱᵐᵖˡ t n;
   max_ordered n t : #(functions max (replicate n t)) = maxⁱᵐᵖˡ t n;
 
